ExistentialRules/Triggers/Basic.lean
@@ -68,6 +68,20 @@ namespace PreTrigger
           rfl
         . exact apply_eq
 
+  theorem result_term_not_in_frontier_image_of_var_not_in_frontier (trg : PreTrigger sig)
+      (disj_index : Fin trg.rule.head.length) (v : sig.V) (v_not_in_frontier : ¬ v ∈ trg.rule.frontier) :
+      ¬ trg.apply_to_var_or_const disj_index.val (VarOrConst.var v) ∈ trg.rule.frontier.map trg.subs := by
+    intro contra
+    apply v_not_in_frontier
+    rw [List.mem_map] at contra
+    rcases contra with ⟨u, u_in_frontier, u_eq⟩
+
+    have := trg.apply_to_var_or_const_injective_of_not_in_frontier disj_index v_not_in_frontier (VarOrConst.var u)
+    rw [VarOrConst.var.injEq] at this
+    rw [this]
+    . exact u_in_frontier
+    . rw [← u_eq, PreTrigger.apply_to_var_or_const_frontier_var]; exact u_in_frontier
+
   abbrev apply_to_function_free_atom (trg : PreTrigger sig) (disjunctIndex : Nat) (atom : FunctionFreeAtom sig) : Fact sig :=
     (trg.apply_to_var_or_const disjunctIndex).apply_generalized_atom atom
 
@@ -173,6 +187,22 @@ namespace PreTrigger
     simp only [fresh_terms_for_head_disjunct, List.mem_map, functional_term_for_var] at t_mem
     rcases t_mem with ⟨_, _, t_mem⟩
     exact ⟨_, _, _, Eq.symm t_mem⟩
+
+  theorem constant_not_mem_fresh_terms_for_head_disjunct {trg : PreTrigger sig} {i : Nat} {lt : i < trg.rule.head.length} :
+      ∀ {c : sig.C}, ¬ .const c ∈ trg.fresh_terms_for_head_disjunct i lt := by
+    intro c c_mem
+    rcases term_functional_of_mem_fresh_terms _ c_mem with ⟨func, ts, arity_ok, eq⟩
+    simp [GroundTerm.const, GroundTerm.func] at eq
+
+  theorem frontier_term_not_mem_fresh_terms_for_head_disjunct {trg : PreTrigger sig} {i : Nat} {lt : i < trg.rule.head.length} :
+      ∀ {t}, t ∈ trg.rule.frontier.map trg.subs -> ¬ t ∈ trg.fresh_terms_for_head_disjunct i lt := by
+    intro t t_frontier t_fresh
+    simp only [fresh_terms_for_head_disjunct, List.mem_map] at t_fresh
+    rcases t_fresh with ⟨v, v_mem, t_fresh⟩; simp only [Rule.existential_vars_for_head_disjunct, List.mem_filter, decide_eq_true_eq] at v_mem
+    apply trg.result_term_not_in_frontier_image_of_var_not_in_frontier ⟨i, lt⟩ v v_mem.right
+    rw [apply_to_var_or_const_non_frontier_var _ _ _ v_mem.right]
+    rw [t_fresh]
+    exact t_frontier
 
   def existential_var_for_fresh_term (trg : PreTrigger sig) (i : Nat) (lt : i < trg.rule.head.length) (t : GroundTerm sig) (t_mem : t ∈ trg.fresh_terms_for_head_disjunct i lt) : sig.V :=
     ((trg.rule.existential_vars_for_head_disjunct i lt).find? (fun v => trg.functional_term_for_var i v = t)).get (by
@@ -548,20 +578,6 @@ namespace PreTrigger
         . apply front; rw [← equiv.left]; exact v_mem
         . exact v_mem
       . simp only [equiv.left]; exact subset
-
-  theorem result_term_not_in_frontier_image_of_var_not_in_frontier (trg : PreTrigger sig)
-      (disj_index : Fin trg.rule.head.length) (v : sig.V) (v_not_in_frontier : ¬ v ∈ trg.rule.frontier) :
-      ¬ trg.apply_to_var_or_const disj_index.val (VarOrConst.var v) ∈ trg.rule.frontier.map trg.subs := by
-    intro contra
-    apply v_not_in_frontier
-    rw [List.mem_map] at contra
-    rcases contra with ⟨u, u_in_frontier, u_eq⟩
-
-    have := trg.apply_to_var_or_const_injective_of_not_in_frontier disj_index v_not_in_frontier (VarOrConst.var u)
-    rw [VarOrConst.var.injEq] at this
-    rw [this]
-    . exact u_in_frontier
-    . rw [← u_eq, PreTrigger.apply_to_var_or_const_frontier_var]; exact u_in_frontier
 
 end PreTrigger
 
